Generalisation of branch unification under assumptions

hol/symb_exec/symb_execLib.sig
@@ -2,10 +2,10 @@ signature symb_execLib =
 sig
   include Abbrev
 
-datatype path_tree = empty | node of int * term * thm * (path_tree list);
+datatype path_tree = empty | node of int * thm * (path_tree list);
 
 val symb_exec:
- (thm * thm -> thm) * thm * (thm -> (term list * thm) option) *
+ (thm * thm -> thm) * thm * (thm -> thm option) *
   (thm -> bool) -> thm -> int -> path_tree * (int * thm * thm) list
 
 end
